sepcomp/Cminor_eff.v
@@ -60,11 +60,12 @@ Inductive cmin_effstep (g: Cminor.genv):  (block -> Z -> bool) ->
       cmin_effstep g (FreeEffect m 0 (f.(fn_stackspace)) sp) (CMin_State f (Stailcall sig a bl) k (Vptr sp Int.zero) e) m
          (CMin_Callstate fd vargs (call_cont k)) m'
 
-  | cmin_effstep_builtin: forall f optid ef bl k sp e m vargs t vres m',
+(* WE DO NOT TREAT BUILTINS *)
+(*| cmin_effstep_builtin: forall f optid ef bl k sp e m vargs t vres m',
       eval_exprlist g sp e m bl vargs ->
       external_call ef g vargs m t vres m' ->
       cmin_effstep g (BuiltinEffect g (ef_sig ef) vargs m) (CMin_State f (Sbuiltin optid ef bl) k sp e) m
-          (CMin_State f Sskip k sp (set_optvar optid vres e)) m'
+          (CMin_State f Sskip k sp (set_optvar optid vres e)) m'*)
 
   | cmin_effstep_seq: forall f s1 s2 k sp e m,
       cmin_effstep g EmptyEffect (CMin_State f (Sseq s1 s2) k sp e) m
@@ -162,8 +163,8 @@ intros.
          apply Mem.unchanged_on_refl.
   split. unfold corestep, coopsem; simpl. econstructor; try eassumption. trivial.
          eapply FreeEffect_free; eassumption.
-  split. unfold corestep, coopsem; simpl. econstructor; try eassumption.
-         eapply ec_builtinEffectPolymorphic; eassumption.
+(*  split. unfold corestep, coopsem; simpl. econstructor; try eassumption.
+         eapply ec_builtinEffectPolymorphic; eassumption.*)
   split. unfold corestep, coopsem; simpl. econstructor; eassumption.
          apply Mem.unchanged_on_refl.
   split. unfold corestep, coopsem; simpl. econstructor; eassumption.
@@ -214,7 +215,7 @@ intros. inv H.
     eexists. eapply cmin_effstep_store; eassumption.
     eexists. eapply cmin_effstep_call; try eassumption. reflexivity.
     eexists. eapply cmin_effstep_tailcall; try eassumption. reflexivity.
-    eexists. eapply cmin_effstep_builtin; eassumption.
+(*    eexists. eapply cmin_effstep_builtin; eassumption.*)
     eexists. eapply cmin_effstep_seq.
     eexists. eapply cmin_effstep_ifthenelse; eassumption.
     eexists. eapply cmin_effstep_loop.
