sepcomp/CminorgenproofEFF.v
@@ -2718,17 +2718,8 @@ Proof.
        PRE TRF MCS _ _ _ _ _ _ optid _ _ MK H H0 H1 EQ EQ1) as [c2' [m2' [mu' [cstepPlus MS]]]].
       exists c2'. exists m2'. exists mu'. 
       intuition. 
-   (*builtin*) admit. (* TODO: case builtin *)
-     (* destruct st1; simpl in *; try inv H. 
-      destruct st1'; simpl in *; try inv H0. 
-      destruct MC as [SMC PRE].
-      inv SMC; simpl in *. 
-      monadInv TR.
-      destruct (MS_step_case_Builtin _ _ _ _ _ _ _ _ _ _ _ _ _ _ _ _ _ 
-       PRE TRF MCS _ _ _ _ _ _ optid args _ MK H1 H2 H3 EQ EQ1) as [c2' [m2' [mu' [cstepPlus MS]]]].
-      exists c2'. exists m2'. exists mu'. 
-      intuition. *)
-  (* seq *)
+   (*builtin*)
+   (* seq *)
      destruct MC as [SMC PRE].
      inv SMC. 
       (*Case 1*) 
@@ -2924,7 +2915,6 @@ Proof.
       intros. destruct H4 as [c2' [m2' [mu' XX]]].
       exists c2', m2', mu'. intuition.
 (* external call - no case*) 
-      
 (* return *) 
       destruct MC as [SMC PRE].
       inv SMC.
@@ -3946,16 +3936,10 @@ induction EFFSTEP; simpl in *.
       exists c2'. exists m2'. exists mu'. 
       intuition.
       exists EmptyEffect. intuition. 
-   (*builtin*) admit. (* TODO: case builtin *)
-      (*destruct st1; simpl in *; try inv H. 
-      destruct st1'; simpl in *; try inv H0. 
-      destruct MC as [SMC PRE].
-      inv SMC; simpl in *. 
-      monadInv TR.
-      destruct (MS_step_case_Builtin _ _ _ _ _ _ _ _ _ _ _ _ _ _ _ _ _ 
-       PRE TRF MCS _ _ _ _ _ _ optid args _ MK H1 H2 H3 EQ EQ1) as [c2' [m2' [mu' [cstepPlus MS]]]].
-      exists c2'. exists m2'. exists mu'. 
-      intuition. *)
+   (*builtin*) 
+      (*destruct (MS_step_case_Builtin _ _ _ _ _ _ _ _ _ _ _ _ _ _ _ _ _ 
+       PRE TRF MCS _ _ _ _ _ _ optid args _ MK H1 H2 H3 EQ EQ1) 
+       as [c2' [m2' [mu' [cstepPlus MS]]]].      intuition. *)
   (* seq *)
      destruct MC as [SMC PRE].
      inv SMC. 
